\documentclass{article}
\usepackage[utf8]{inputenc}
\usepackage{amsmath}
\DeclareMathOperator{\Tr}{Tr}
\usepackage{physics}
\usepackage{xcolor}

\title{Analytical Solution of Asteroid ODEs}
\author{Eros433}
\date{\today}

\begin{document}

\maketitle

\noindent\begin{minipage}{.5\linewidth}
\begin{align*}
\begin{cases}
\frac{{\rm d}v}{{\rm d}t}&=\frac{-c_{{\rm D}}\,\rho_{\rm a}(z)\,A\,v^{2}}{2\,m}+g\,{\rm sin}(\theta)\\[0.3cm]
\frac{{\rm d}m}{{\rm d}t}&=\frac{-c_{{\rm H}}\,\rho_{\rm a}(z)}{2\,Q}\\[0.3cm]
\frac{{\rm d}\theta}{{\rm d}t}&=\frac{g\,{\rm cos}(\theta)}{v}-\frac{c_{\rm L}\,\rho_{{\rm a}(z)}\,A\,v}{2\,m}-\frac{v\,{\rm cos}(\theta)}{R_{\rm P}+z}\\[0.3cm]
\frac{{\rm d}z}{{\rm d}t}&=-v\,{\rm sin}(\theta)\\[0.5cm]
\frac{{\rm d}x}{{\rm d}t}&=\frac{v\,{\rm cos}(\theta)}{1+\frac{z}{R_{\rm P}}}\\[0.3cm]
\rho_a(z)&=\rho_0\,e^{-\frac{z}{H}}\\[0.3cm]
\frac{{\rm d}r}{{\rm d}t}&=\left[\frac{7}{2}\,\alpha\frac{\rho_{\rm a}}{\rho_{{\rm m}}}\right]^{\frac{1}{2}}v\\[0.3cm]
\rho_{\rm a}(z)\,v^{\rm 2}&=\sigma_{\rm 0}
\end{cases}
\rightarrow
\end{align*}
\end{minipage}%
\begin{minipage}{.5\linewidth}
\begin{align*}
\begin{cases}
\frac{{\rm d}v}{{\rm d}t}&=\frac{-c_{{\rm D}}\,\rho_{\rm a}(z)\,A\,v^2}{2\,m}\\[0.3cm]
\frac{{\rm d}m}{{\rm d}t}&=0\\[0.3cm]
\frac{{\rm d}\theta}{{\rm d}t}&=0\\[0.3cm]
\frac{{\rm d}z}{{\rm d}t}&=-v\,{\rm sin}(\theta)\\[0.3cm]
\frac{{\rm d}x}{{\rm d}t}&=v\,{\rm cos}(\theta)\\[0.3cm]
\rho_a(z)&=\rho_0\,e^{-\frac{z}{H}}\\[0.3cm]
\frac{{\rm d}r}{{\rm d}t}&=0\\[0.3cm]
\end{cases}
\end{align*}
\end{minipage}
\\[0.5cm]
$\rightarrow m={\rm const.},\theta={\rm const.},r={\rm const.}$\\[0.3cm]
$\{\frac{{\rm d}v}{{\rm d}t}=\frac{-c_{\rm D}\,\rho_{\rm a}(z)\,A\,v^{\rm 2}}{2\,m},\frac{{\rm d}z}{{\rm d}t}=-v\,{\rm sin}(\theta)\}$\\[0.2cm]
$\{{\rm d}t=\frac{2\,m}{-c_{\rm D}\,\rho_{\rm a}(z)\,A\,v^{\rm 2}}{\rm d}v,{\rm d}z=-v\,{\rm sin}(\theta){\rm d}t\}$\\[0.3cm]
${\rm d}z=\frac{2\,m\,{\rm sin}(\theta)}{c_{\rm D}\,A\,\rho_a(z)}\frac{{\rm d}v}{v}$\\[0.3cm]
$\displaystyle\int_{z_0}^{z}{\rho_{\rm a}(z){\rm d}z}=\frac{2\,m\,{\rm sin}(\theta)}{c_{\rm D}\,A}\,\int_{v_0}^{v}\frac{{\rm d}v}{v}$\\[0.3cm]
${\rm ln}(\frac{v}{v_0})=\frac{c_{\rm D}\,A\,H\,\rho_0}{2\,m\,{\rm sin}(\theta)}\left(e^{-\frac{z_0}{H}}-e^{-\frac{z}{H}}\right)$\\[0.3cm]
$v=v_0\,{\rm exp}\left(\frac{c_{\rm D}\,A\,H\,\rho_0}{2\,m\,{\rm sin}(\theta)}\left(e^{-\frac{z_0}{H}}-e^{-\frac{z}{H}}\right)\right)$\\[0.3cm]
\end{document}